fix heap_lang/total_adequacy

theories/heap_lang/adequacy.v
@@ -4,17 +4,17 @@ From iris.heap_lang Require Import proofmode notation proph_map.
 From iris.proofmode Require Import tactics.
 Set Default Proof Using "Type".
 
-Class heap_prophPreG Σ := HeapProphPreG {
-  heap_proph_preG_iris :> invPreG Σ;
-  heap_proph_preG_heap :> gen_heapPreG loc val Σ;
-  heap_proph_preG_proph :> proph_mapPreG proph val Σ
+Class heapPreG Σ := HeapPreG {
+  heap_preG_iris :> invPreG Σ;
+  heap_preG_heap :> gen_heapPreG loc val Σ;
+  heap_preG_proph :> proph_mapPreG proph val Σ
 }.
 
 Definition heapΣ : gFunctors := #[invΣ; gen_heapΣ loc val; proph_mapΣ proph val].
-Instance subG_heapPreG {Σ} : subG heapΣ Σ → heap_prophPreG Σ.
+Instance subG_heapPreG {Σ} : subG heapΣ Σ → heapPreG Σ.
 Proof. solve_inG. Qed.
 
-Definition heap_adequacy Σ `{heap_prophPreG Σ} s e σ φ :
+Definition heap_adequacy Σ `{heapPreG Σ} s e σ φ :
   (∀ `{heapG Σ}, WP e @ s; ⊤ {{ v, ⌜φ v⌝ }}%I) →
   adequate s e σ (λ v _, φ v).
 Proof.
